cvc5Test/Unit/ApiResult.lean
@@ -13,15 +13,16 @@ test![TestApiBlackResult, isNull] do
   -- lean API does not expose null results
   assertTrue true
 
-test![TestApiBlackResult, equalHash] solver => do
-  let u ← mkUninterpretedSort "u"
+test![TestApiBlackResult, equalHash] tm => do
+  let solver ← Solver.new tm
+  let u ← tm.mkUninterpretedSort "u"
   let x ← solver.declareFun "x" #[] u
-  let x_eq_x ← mkTerm .EQUAL #[x, x]
+  let x_eq_x ← tm.mkTerm .EQUAL #[x, x]
   solver.assertFormula x_eq_x
   -- skipping null-result-related checks
   let res1 ← solver.checkSat
   let res2 ← solver.checkSat
-  solver.assertFormula (← mkTerm .NOT #[x_eq_x])
+  solver.assertFormula (← tm.mkTerm .NOT #[x_eq_x])
   let res3 ← solver.checkSat
   assertEq res1 res2
   assertNe res1 res3
@@ -33,10 +34,11 @@ test![TestApiBlackResult, equalHash] solver => do
   assertNe res1.hash res3.hash
   assertNe res2.hash res3.hash
 
-test![TestApiBlackResult, isSat] solver => do
-  let u ← mkUninterpretedSort "u"
+test![TestApiBlackResult, isSat] tm => do
+  let solver ← Solver.new tm
+  let u ← tm.mkUninterpretedSort "u"
   let x ← solver.declareFun "x" #[] u
-  solver.assertFormula (← mkTerm .EQUAL #[x, x])
+  solver.assertFormula (← tm.mkTerm .EQUAL #[x, x])
   let res ← solver.checkSat
   assertTrue res.isSat
   assertFalse res.isUnsat
@@ -47,10 +49,11 @@ test![TestApiBlackResult, isSat] solver => do
   assertEq ue.toString "UNKNOWN_REASON"
   assertEq res.getUnknownExplanation? none
 
-test![TestApiBlackResult, isUnsat] solver => do
-  let u ← mkUninterpretedSort "u"
+test![TestApiBlackResult, isUnsat] tm => do
+  let solver ← Solver.new tm
+  let u ← tm.mkUninterpretedSort "u"
   let x ← solver.declareFun "x" #[] u
-  solver.assertFormula (← mkTerm .NOT #[← mkTerm .EQUAL #[x, x]])
+  solver.assertFormula (← tm.mkTerm .NOT #[← tm.mkTerm .EQUAL #[x, x]])
   let res ← solver.checkSat
   assertFalse res.isSat
   assertTrue res.isUnsat
@@ -61,16 +64,17 @@ test![TestApiBlackResult, isUnsat] solver => do
   assertEq ue.toString "UNKNOWN_REASON"
   assertEq res.getUnknownExplanation? none
 
-test![TestApiBlackResult, isUnknown] solver => do
+test![TestApiBlackResult, isUnknown] tm => do
+  let solver ← Solver.new tm
   solver.setLogic "QF_NIA"
   solver.setOption "incremental" "false"
   solver.setOption "solve-real-as-int" "true"
-  let realSort ← getRealSort
+  let realSort ← tm.getRealSort
   let x ← solver.declareFun "x" #[] realSort
-  let zero := ← mkReal 0
-  let one := ← mkReal 1
-  solver.assertFormula (← mkTerm .LT #[zero, x])
-  solver.assertFormula (← mkTerm .LT #[x, one])
+  let zero := ← tm.mkReal 0
+  let one := ← tm.mkReal 1
+  solver.assertFormula (← tm.mkTerm .LT #[zero, x])
+  solver.assertFormula (← tm.mkTerm .LT #[x, one])
   let res ← solver.checkSat
   assertFalse res.isSat
   assertFalse res.isUnsat
