cvc5Test/Unit/ApiSkolemId.lean
@@ -8,13 +8,13 @@ import cvc5Test.Init
 namespace cvc5.Test
 
 test![TestApiBlackSkolemId, skolemIdToString] do
-  for idx in [SkolemId.INTERNAL.ctorIdx : SkolemId.NONE.ctorIdx] do
+  for idx in [SkolemId.INTERNAL.toCtorIdx : SkolemId.NONE.toCtorIdx] do
     let si := SkolemId.ofNat idx
     -- if this assertion fails, the switch in `enum_to_string.cpp` is missing id `si`.
     assertNe si.toString "?"
 
 test![TestApiBlackSkolemId, skolemIdHash] do
-  for idx in [SkolemId.INTERNAL.ctorIdx : SkolemId.NONE.ctorIdx] do
+  for idx in [SkolemId.INTERNAL.toCtorIdx : SkolemId.NONE.toCtorIdx] do
     let si := SkolemId.ofNat idx
-    assertEq si.hash ⟨si.ctorIdx⟩
+    assertEq si.hash ⟨si.toCtorIdx⟩
   assertNe SkolemId.PURIFY.hash SkolemId.INTERNAL.hash
