cvc5Test/Unit/ApiTermManager.lean
@@ -11,109 +11,109 @@ namespace cvc5.Test
 
 open Env
 
-test! do
-  let _ ← getBooleanSort
+test! tm => do
+  let _ ← tm.getBooleanSort
 
-test! do
-  let _ ← getIntegerSort
+test! tm => do
+  let _ ← tm.getIntegerSort
 
-test! do
-  let _ ← getRealSort
+test! tm => do
+  let _ ← tm.getRealSort
 
-test! do
-  let _ ← getRegExpSort
+test! tm => do
+  let _ ← tm.getRegExpSort
 
-test! do
-  let _ ← getStringSort
+test! tm => do
+  let _ ← tm.getStringSort
 
-test! do
-  let _ ← getRoundingModeSort
+test! tm => do
+  let _ ← tm.getRoundingModeSort
 
-test! do
-  let boolSort ← getBooleanSort
-  let intSort ← getIntegerSort
-  let realSort ← getRealSort
-  let bvSort ← mkBitVectorSort 32
+test! tm => do
+  let boolSort ← tm.getBooleanSort
+  let intSort ← tm.getIntegerSort
+  let realSort ← tm.getRealSort
+  let bvSort ← tm.mkBitVectorSort 32
 
   let size ←
     bvSort.getBitVectorSize
     |> assertOk
   assertEq size 32
 
-  mkArraySort boolSort boolSort
+  tm.mkArraySort boolSort boolSort
   |> assertOkDiscard
-  mkArraySort intSort intSort
+  tm.mkArraySort intSort intSort
   |> assertOkDiscard
-  mkArraySort realSort realSort
+  tm.mkArraySort realSort realSort
   |> assertOkDiscard
-  mkArraySort bvSort bvSort
+  tm.mkArraySort bvSort bvSort
   |> assertOkDiscard
-  mkArraySort boolSort intSort
+  tm.mkArraySort boolSort intSort
   |> assertOkDiscard
-  mkArraySort realSort bvSort
+  tm.mkArraySort realSort bvSort
   |> assertOkDiscard
 
-  let fpSort ← mkFloatingPointSort 3 5
-  mkArraySort fpSort fpSort
+  let fpSort ← tm.mkFloatingPointSort 3 5
+  tm.mkArraySort fpSort fpSort
   |> assertOkDiscard
-  mkArraySort bvSort fpSort
+  tm.mkArraySort bvSort fpSort
   |> assertOkDiscard
   -- already tested, probably a typo in the original test
-  mkArraySort boolSort boolSort
+  tm.mkArraySort boolSort boolSort
   |> assertOkDiscard
 
-  mkArraySort (← getBooleanSort) (← getIntegerSort)
+  tm.mkArraySort (← tm.getBooleanSort) (← tm.getIntegerSort)
   |> assertOkDiscard
 
-test! do
-  mkBitVectorSort 32
+test! tm => do
+  tm.mkBitVectorSort 32
   |> assertOkDiscard
-  mkBitVectorSort 0
+  tm.mkBitVectorSort 0
   |> assertError "invalid argument '0' for 'size', expected size > 0"
 
-test! do
-  mkFiniteFieldSort 31
+test! tm => do
+  tm.mkFiniteFieldSort 31
   |> assertOkDiscard
-  mkFiniteFieldSort 6
+  tm.mkFiniteFieldSort 6
   |> assertError "invalid argument '6' for 'modulus', expected modulus is prime"
 
-  mkFiniteFieldSort 1100101 2
+  tm.mkFiniteFieldSort 1100101 2
   |> assertOkDiscard
-  mkFiniteFieldSort 10202 3
+  tm.mkFiniteFieldSort 10202 3
   |> assertOkDiscard
-  mkFiniteFieldSort 401 5
+  tm.mkFiniteFieldSort 401 5
   |> assertOkDiscard
-  mkFiniteFieldSortOfString "791a" 11
+  tm.mkFiniteFieldSortOfString "791a" 11
   |> assertOkDiscard
-  mkFiniteFieldSortOfString "970f" 16
+  tm.mkFiniteFieldSortOfString "970f" 16
   |> assertOkDiscard
-  mkFiniteFieldSortOfString "8CC5" 16
+  tm.mkFiniteFieldSortOfString "8CC5" 16
   |> assertOkDiscard
 
-  mkFiniteFieldSort 1100100 2
+  tm.mkFiniteFieldSort 1100100 2
   |> assertError "invalid argument '1100100' for 'modulus', expected modulus is prime"
-  mkFiniteFieldSort 10201 3
+  tm.mkFiniteFieldSort 10201 3
   |> assertError "invalid argument '10201' for 'modulus', expected modulus is prime"
-  mkFiniteFieldSort 400 5
+  tm.mkFiniteFieldSort 400 5
   |> assertError "invalid argument '400' for 'modulus', expected modulus is prime"
-  mkFiniteFieldSort 7919 11
+  tm.mkFiniteFieldSort 7919 11
   |> assertError "invalid argument '7919' for 'modulus', expected modulus is prime"
-  mkFiniteFieldSortOfString "970e" 16
+  tm.mkFiniteFieldSortOfString "970e" 16
   |> assertError "invalid argument '970e' for 'modulus', expected modulus is prime"
-  mkFiniteFieldSortOfString "8CC4" 16
+  tm.mkFiniteFieldSortOfString "8CC4" 16
   |> assertError "invalid argument '8CC4' for 'modulus', expected modulus is prime"
 
-test! do
-  mkFloatingPointSort 4 8
+test! tm => do
+  tm.mkFloatingPointSort 4 8
   |> assertOkDiscard
 
-  mkFloatingPointSort 0 8
+  tm.mkFloatingPointSort 0 8
   |> assertError "invalid argument '0' for 'exp', expected exponent size > 1"
-  mkFloatingPointSort 4 0
+  tm.mkFloatingPointSort 4 0
   |> assertError "invalid argument '0' for 'sig', expected significand size > 1"
-  mkFloatingPointSort 1 8
+  tm.mkFloatingPointSort 1 8
   |> assertError "invalid argument '1' for 'exp', expected exponent size > 1"
-  mkFloatingPointSort 4 1
+  tm.mkFloatingPointSort 4 1
   |> assertError "invalid argument '1' for 'sig', expected significand size > 1"
 
 
@@ -126,71 +126,71 @@ Datatype-related tests
 -/
 
 
-test! do
+test! tm => do
   let uf ←
-    mkUninterpretedSort "u"
+    tm.mkUninterpretedSort "u"
     |> assertOk
-  let int ← getIntegerSort
+  let int ← tm.getIntegerSort
   let funSort ←
-    mkFunctionSort #[uf] int
+    tm.mkFunctionSort #[uf] int
     |> assertOk
 
   -- function arguments are allowed
-  mkFunctionSort #[funSort] int
+  tm.mkFunctionSort #[funSort] int
   |> assertOkDiscard
   -- non-first-class arguments are not allowed
-  let reSort ← getRegExpSort
-  mkFunctionSort #[reSort] int
+  let reSort ← tm.getRegExpSort
+  tm.mkFunctionSort #[reSort] int
   |> assertError
     "invalid domain sort in 'sorts' at index 0, expected first-class sort as domain sort"
   --
-  mkFunctionSort #[int] funSort
+  tm.mkFunctionSort #[int] funSort
   |> assertError
     "invalid argument '(-> u Int)' for 'codomain', expected non-function sort as codomain sort"
   --
-  mkFunctionSort #[uf, int] int
+  tm.mkFunctionSort #[uf, int] int
   |> assertOkDiscard
 
   let funSort2 ←
-    mkFunctionSort #[← mkUninterpretedSort "u"] (← getBooleanSort)
+    tm.mkFunctionSort #[← tm.mkUninterpretedSort "u"] (← tm.getBooleanSort)
     |> assertOk
   --
-  mkFunctionSort #[funSort2, uf] int
+  tm.mkFunctionSort #[funSort2, uf] int
   |> assertOkDiscard
   --
-  mkFunctionSort #[int, uf] funSort2
+  tm.mkFunctionSort #[int, uf] funSort2
   |> assertError
     "invalid argument '(-> u Bool)' for 'codomain', expected non-function sort as codomain sort"
 
-  let bool ← getBooleanSort
+  let bool ← tm.getBooleanSort
   let sorts1 := #[bool, int, int]
   let sorts2 := #[bool, int]
 
-  mkFunctionSort sorts2 int
+  tm.mkFunctionSort sorts2 int
   |> assertOkDiscard
-  mkFunctionSort sorts1 int
+  tm.mkFunctionSort sorts1 int
   |> assertOkDiscard
 
   -- At this point the original test creates a new `TermManager` and checks that some constructors
   -- fail because the manager is not a singleton anymore. But we don't have that problem.
 
-test! do
-  mkParamSort "T"
+test! tm => do
+  tm.mkParamSort "T"
   |> assertOkDiscard
-  mkParamSort ""
+  tm.mkParamSort ""
   |> assertOkDiscard
 
-test! do
-  mkPredicateSort #[← getIntegerSort]
+test! tm => do
+  tm.mkPredicateSort #[← tm.getIntegerSort]
   |> assertOkDiscard
-  mkPredicateSort #[]
+  tm.mkPredicateSort #[]
   |> assertError
     "invalid size of argument 'sorts', expected at least one parameter sort for predicate sort"
   -- function as arguments are allowed
-  let funSort ← mkFunctionSort #[← mkUninterpretedSort "u"] (← getIntegerSort)
-  mkPredicateSort #[← getIntegerSort, funSort]
+  let funSort ← tm.mkFunctionSort #[← tm.mkUninterpretedSort "u"] (← tm.getIntegerSort)
+  tm.mkPredicateSort #[← tm.getIntegerSort, funSort]
   |> assertOkDiscard
-  mkPredicateSort #[← getIntegerSort]
+  tm.mkPredicateSort #[← tm.getIntegerSort]
   |> assertOkDiscard
 
   -- At this point the original test creates a new `TermManager` and checks that some constructors
